Sorry-free!

MemoNat.lean
@@ -1,6 +1,7 @@
 -- This intentionally only uses std, not mathlib
 import Std.Data.Array.Lemmas
 import Std.Data.Fin.Basic
+import Std.Data.Fin.Lemmas
 import Std.Tactic.Congr
 import MemoNat.DArray
 
@@ -67,59 +68,230 @@ protected theorem get_push {C n} (a : DSArray n C) (i : Nat) (hi : i < n + 1) (x
       cases ha
       rfl
 
+protected def ofFn {C} (n : Nat) (f : (i : Fin n) → C i) : DSArray n C :=
+  ⟨.ofFn n f, DArray.size_ofFn n f⟩
+
+@[simp]
+protected theorem get_ofFn  {C : Nat → Sort _} (n : Nat) (f : (i : Fin n) → C i)
+    (i : Fin n) : (DSArray.ofFn n f).get i = f i := DArray.get_ofFn _ _ _
+
+theorem Array.get_pop {α} (a : Array α) (i : Fin a.pop.size) :
+  a.pop.get i = a.get (i.castLE (a.size_pop ▸ Nat.sub_le _ _ )) := by
+    cases i with | _ i hi =>
+    cases a with | _ xs =>
+    unfold Array.pop Array.size Array.get at *
+    dsimp
+    dsimp at hi
+    induction i generalizing xs
+    case zero =>
+      cases xs
+      case nil => rfl
+      case cons x xs =>
+        cases xs
+        · simp at hi
+        · simp
+    case succ i IH =>
+      cases xs
+      case nil => rfl
+      case cons x xs =>
+        cases xs
+        case nil =>
+          simp at hi
+          exfalso
+          apply Nat.not_lt_zero _ hi
+        case cons y ys =>
+          apply IH
+
+def _root_.DArray.pop {C} (a : DArray C) : DArray C :=
+  ⟨a.arr.pop, by
+    intro i
+    cases a with | _ a ha =>
+    rw [Array.get_pop]
+    apply ha ⟩
+
+theorem _root_.DArray.size_pop {C} (a : DArray C) :
+  a.pop.size = a.size - 1 := Array.size_pop _
+
+@[simp]
+theorem _root_.DArray.get_pop {C} (a : DArray C) (i : Fin a.pop.size):
+  a.pop.get i = a.get (i.castLE (a.size_pop ▸ Nat.sub_le _ _)) := by
+    unfold DArray.pop DArray.get
+    apply Any.eq_rec_val
+    simp only [Fin.coe_castLE, Any.mk_eq_rec', Array.get_pop]
+
+def pop {C n} (a : DSArray (n + 1) C) : DSArray n C :=
+  ⟨a.val.pop, by rw [DArray.size_pop, a.2]; rfl⟩
+
+@[simp]
+theorem _root_.DSArray.get_pop {C n} (a : DSArray (n + 1) C) (i : Fin n):
+    a.pop.get i = a.get i.castSucc := DArray.get_pop _ _
+
+def of_below {C} : {n : Nat} → @Nat.below C n → DSArray n C
+  | 0, .unit => .empty 0
+  | n + 1, ⟨⟨x,y⟩,.unit⟩ => (@of_below C n y).push x
+
+def below_ofFn {C} : (n : Nat) → (f : (i : Fin n) → C i) → @Nat.below C n
+  | 0, _ => .unit
+  | n+1, f => ⟨⟨f (Fin.last n), below_ofFn n (fun i => f i.castSucc)⟩,.unit⟩
+
+def to_below {C n} (a : DSArray n C) : @Nat.below C n :=
+  below_ofFn n a.get
+
+theorem to_below_succ {C n} (a : DSArray (n + 1) C) :
+  a.to_below = ⟨⟨a.get (Fin.last n), a.pop.to_below⟩, .unit⟩ := by
+  cases n <;> simp only [to_below, ← Fin.succ_last, below_ofFn, get_pop]
+
+@[ext]
+theorem ext {C n} (a b : DSArray n C)
+    (h₂ : (i : Nat) → (hi : i < n) → a.get ⟨i, hi⟩ = b.get ⟨i, hi⟩)
+    : a = b := by
+  cases a with | _ a ha =>
+  cases b with | _ b hb =>
+  suffices a = b by simp [this]
+  apply DArray.ext _ _ (ha.trans hb.symm)
+  intro i hi₁ _hi₂ 
+  exact h₂ i (ha ▸ hi₁)
+
+@[simp]
+theorem pop_ofFn {C : Nat → Sort u} (n : Nat) (g : (i : Fin (n+1)) → C i) :
+    DSArray.pop (DSArray.ofFn (Nat.succ n) g) = DSArray.ofFn n (fun i => g i.castSucc) := by
+  ext i hi
+  simp
+
 end DSArray
 
 namespace NatMemo
 
 protected def dmemoVec {C : Nat → Sort u} (cap : Nat)
-    (f : (n : Nat) → (∀ i, i < n → C i) → C n) :
+    (f : (n : Nat) → DSArray n C → C n) :
     (n : Nat) → DSArray n C
   | 0 => .empty cap
   | n + 1 =>
     let v := NatMemo.dmemoVec cap f n
-    v.push (f n (fun i ih => v.get ⟨i, ih⟩))
+    v.push (f n v)
+
+theorem dmemoVec_eq_ofFn {C : Nat → Sort u}
+    (c : Nat)
+    (g : ∀ n, C n)
+    (f : (n : Nat) → DSArray n C → C n)
+    (h : ∀ n, f n (.ofFn (n := n) (fun i => g i)) = g n)
+    (n : Nat) : NatMemo.dmemoVec c f n = .ofFn (n:=n) (fun i => g i) := by
+  induction n
+  · case zero => rfl
+  · case succ n IH => 
+    unfold NatMemo.dmemoVec
+    simp only
+    rw [IH]
+    ext i hi
+    dsimp
+    rw [DSArray.get_push, DSArray.get_ofFn]
+    split
+    case inl hn =>
+      simp only [DSArray.get_ofFn]
+    case inr hn =>
+      have i_eq_n : i = n := Nat.le_antisymm (Nat.lt_succ.1 hi) (Nat.not_lt.1 hn)
+      rcases i_eq_n
+      simp only [DSArray.get_ofFn, h]
 
 def dmemo {C : Nat → Sort u} (f : (n : Nat) → (∀ i, i < n → C i) → C n) (n : Nat) : C n :=
-  (NatMemo.dmemoVec (n + 1) f (n + 1)).get ⟨n, Nat.le_refl _⟩
+  (NatMemo.dmemoVec (n + 1) (fun n a => f n (fun i ih => a.get ⟨i, ih⟩)) (n + 1)
+  ).get ⟨n, Nat.le_refl _⟩
 
-theorem dmemoVec_spec {C : Nat → Sort u}
-  (g : ∀ n, C n)
-  (f : (n : Nat) → (∀ i, i < n → C i) → C n)
-  (h : ∀ n, f n (fun i _ => g i) = g n)
-  n : ∀ c i hi, (NatMemo.dmemoVec c f n).get ⟨i, hi⟩ = g i := by
-    induction n
-    case zero => 
-      intro c i hi
-      cases hi
-    case succ n ih =>
-      intro c i hi
-      rw [NatMemo.dmemoVec]
-      apply Eq.trans (DSArray.get_push _ _ _ _)
-      split
-      case inl hn =>
-        apply ih
-      case inr hn =>
-        have i_eq_n : i = n := Nat.le_antisymm (Nat.lt_succ.1 hi) (Nat.not_lt.1 hn)
-        rcases i_eq_n
-        rw [<- h]
-        simp only
-        congr with i hi'
-        apply ih
 
 theorem dmemo_spec {C : Nat → Sort u}
     (g : ∀ n, C n)
     (f : (n : Nat) → (∀ i, i < n → C i) → C n)
     (h : ∀ n, f n (fun i _ => g i) = g n) :
-    g = dmemo f :=
-  funext (fun _ => (dmemoVec_spec g f h _ _ _ _).symm)
-
+    g = dmemo f := by
+  ext n
+  unfold dmemo
+  rw [dmemoVec_eq_ofFn _ g]
+  · simp only [DSArray.get_ofFn]
+  · intro n' 
+    simp only [DSArray.get_ofFn, h]
 
 theorem fix_eq_dmemo {C : Nat → Sort u}
-  (f : (n : Nat) → (∀ i, i < n → C i) → C n)
-  : WellFounded.fix (invImage (fun a => sizeOf a) instWellFoundedRelation).2 f = dmemo f := by
-    apply dmemo_spec
+    (f : (n : Nat) → (∀ i, i < n → C i) → C n) :
+    WellFounded.fix (invImage (fun a => sizeOf a) instWellFoundedRelation).2 f = dmemo f := by
+  apply dmemo_spec
+  intro n
+  apply (WellFounded.fix_eq _ _ _).symm
+
+def dmemo_below {C : Nat → Sort u}
+    (f : (n : Nat) → @Nat.below C n → C n)
+    (n : Nat) : C n :=
+  (NatMemo.dmemoVec (n + 1) (fun n a => f n a.to_below) (n + 1)).get ⟨n, Nat.le_refl _⟩
+
+def below_ofFn {C : Nat → Sort u} (g : ∀ n, C n) : (n : Nat) → @Nat.below C n
+  | 0 => PUnit.unit
+  | n+1 => ⟨⟨g n, below_ofFn g n⟩,.unit⟩
+
+
+
+theorem DSArray.to_below_ofFn_eq_below_ofFn {C : Nat → Sort u} (n : Nat) (g : (i : Nat) → C i)  :
+    DSArray.to_below (DSArray.ofFn n (fun i => g i)) = below_ofFn g n := by
+  induction n
+  · case zero => rfl
+  · case succ n IH => 
+    rw [DSArray.to_below_succ]
+    dsimp [below_ofFn]
+    rw [DSArray.get_ofFn]
+    congr
+    rw [DSArray.pop_ofFn]
+    exact IH
+
+theorem dmemo_below_spec {C : Nat → Sort u}
+    (g : ∀ n, C n)
+    (f : (n : Nat) → @Nat.below C n → C n)
+    (h : ∀ n, f n (below_ofFn g n) = g n) :
+    g = dmemo_below f := by
+  ext n
+  unfold dmemo_below
+  rw [dmemoVec_eq_ofFn _ g]
+  · simp only [DSArray.get_ofFn]
+  · intro n' 
+    rw [DSArray.to_below_ofFn_eq_below_ofFn n']
+    apply h
+
+noncomputable
+def brecOn_recurser {C : Nat → Sort u} (f : (n : Nat) → @Nat.below C n → C n)  :
+    (n : Nat) → PProd (C n) (@Nat.below C n) :=
+  Nat.rec (motive := fun n => PProd (C n) (Nat.below n))
+    ⟨f Nat.zero PUnit.unit, PUnit.unit ⟩
+    fun n ih => ⟨f (Nat.succ n) ⟨ih, PUnit.unit⟩, ⟨ih, PUnit.unit ⟩⟩
+
+theorem brecOn_eq_brecOn_recurser
+     {C : Nat → Sort u} (f : (n : Nat) → @Nat.below C n → C n) (n : Nat) :
+     @Nat.brecOn C n f = (brecOn_recurser f n).1 := rfl
+
+theorem brecOn_recurser_eq {C : Nat → Sort u} (f : (n : Nat) → @Nat.below C n → C n) :
+  (n : Nat) → brecOn_recurser f n =
+    ⟨f n (brecOn_recurser f n).2,(brecOn_recurser f n).2⟩ := by
+  intro n; cases n <;> rfl
+
+theorem recurser_two_eq {C : Nat → Sort u} (f : (n : Nat) → @Nat.below C n → C n) (n : Nat) :
+  (brecOn_recurser f n).2 = below_ofFn (fun n => @Nat.brecOn C n f) n := by
+  induction n
+  · case zero => rfl
+  · case succ n IH =>
+    unfold brecOn_recurser
+    show (⟨brecOn_recurser f n, PUnit.unit⟩ = (_ : PProd _ _))
+    rw [brecOn_recurser_eq]
+    congr
+    simp only [brecOn_eq_brecOn_recurser]
+    rw [brecOn_recurser_eq]
+
+theorem brecOn_eq {C : Nat → Sort u} 
+    (f : (n : Nat) → @Nat.below C n → C n)
+    (n : Nat) : @Nat.brecOn C n f = f n (below_ofFn (fun n => @Nat.brecOn C n f) n) := by
+  rw [brecOn_eq_brecOn_recurser, brecOn_recurser_eq, recurser_two_eq]
+
+theorem brecOn_eq_dmemo_below {C : Nat → Sort u}
+    (f : (n : Nat) → @Nat.below C n → C n)
+    : (fun n => @Nat.brecOn C n f) = dmemo_below f := by
+    apply dmemo_below_spec
     intro n
-    apply (WellFounded.fix_eq _ _ _).symm
+    exact (brecOn_eq f n).symm
 
 def memo {α : Sort u} (f : (n : Nat) → (∀ i, i < n → α) → α) (n : Nat) : α :=
   dmemo f n
@@ -128,23 +300,12 @@ theorem memo_spec {α : Sort u}
     (g : Nat → α)
     (f : (n : Nat) → (∀ i, i < n → α) → α)
     (h : ∀ n, f n (fun i _ => g i) = g n) :
-    g = dmemo f :=
+    g = memo f :=
   dmemo_spec g f h
 
 
 theorem fix_eq_memo {α} (f : (n : Nat) → (∀ i, i < n → α) → α) :
     WellFounded.fix (invImage (fun a => sizeOf a) instWellFoundedRelation).2 f = memo f :=
   fix_eq_dmemo f
-
-
-/-
-theorem Brec_eq_memo {α}
-  (f : (n : Nat) → Nat.below n → α)
-  : (fun n => Nat.brecOn n f) = memo f := by
-    apply memo_spec
-    intro n
-    apply (WellFounded.fix_eq _ _ _).symm
--/
-
 
 end NatMemo
