MemoNat/DArray.lean
@@ -16,9 +16,22 @@ protected abbrev Any.Sort : Any → Sort _
 protected abbrev Any.val : (a : Any) → a.Sort
 | mk x => x
 
-theorem Any.congr {a₁ a₂ : Any}  (h : a₁ = a₂) {α : Sort u} {h₁ : a₁.Sort = α}
+-- theorem Any.congr {a₁ a₂ : Any} (h : a₁ = a₂) {α : Sort u} {h₁ : a₁.Sort = α}
+--     {h₂ : a₂.Sort = α} :
+--     h₁ ▸ a₁.val = h₂ ▸ a₂.val := by induction h; rfl
+
+@[simp]
+theorem Any.eq_rec_val_iff {a₁ a₂ : Any} {α : Sort u} {h₁ : a₁.Sort = α}
     {h₂ : a₂.Sort = α} :
-    h₁ ▸ a₁.val = h₂ ▸ a₂.val := by induction h; rfl
+    (h₁ ▸ a₁.val = h₂ ▸ a₂.val) ↔ (a₁ = a₂) := by
+    constructor
+    · intro h
+      cases a₁ with | @mk α₁ x =>
+      cases a₂ with | @mk α₂ y =>
+      cases h₁
+      cases h₂
+      exact congrArg Any.mk h
+    · intro h; induction h; rfl
 
 theorem Any.rw {a₁ a₂ : Any}  (h : a₁ = a₂) {α : Sort u} {h₁ : a₁.Sort = α} :
     h₁ ▸ a₁.val = (h ▸ h₁) ▸ a₂.val := by induction h; rfl
@@ -92,5 +105,39 @@ theorem get_push {C} (a : DArray C) (x : C a.size) (i : Fin (a.push x).size) :
     rfl
   case inr hi2 =>
     simp only [get, Array.get, Any.mk_eq_rec', DArray.size, Any.mk_eq_rec ]
+ 
+protected def ofFn {C} (n : Nat) (f : (i : Fin n) → C i) : DArray C :=
+  ⟨ .ofFn fun i => Any.mk (f i),
+    by intro i; rw [Array.get_eq_getElem, Array.getElem_ofFn] ⟩
+
+protected theorem size_ofFn  {C : Nat → Sort _} (n : Nat) (f : (i : Fin n) → C i) :
+  (DArray.ofFn n f).size = n := by
+  dsimp [DArray.size, DArray.ofFn]
+  exact Array.size_ofFn _
+
+protected theorem get_ofFn {C : Nat → Sort _} (n : Nat) (f : (i : Fin n) → C i)
+    (i : Fin (size (DArray.ofFn n f))) : (DArray.ofFn n f).get i =
+    f (i.cast (DArray.size_ofFn n f)) := by
+  dsimp [DArray.get, DArray.size, DArray.ofFn]
+  apply Any.eq_rec_val
+  simp only [Array.getElem_ofFn, Any.mk.injEq, heq_eq_eq, true_and]
+  rfl
+
+theorem ext {C} (a b : DArray C)
+    (h₁ : a.size = b.size)
+    (h₂ : (i : Nat) → (hi₁ : i < a.size) → (hi₂ : i < b.size) → a.get ⟨i, hi₁⟩ = b.get ⟨i, hi₂⟩)
+    : a = b := by
+  cases a with | _ a ha =>
+  cases b with | _ b hb =>
+  simp only [mk.injEq]
+  apply Array.ext
+  · exact h₁
+  · clear h₁
+    intro i hi₁ hi₂
+    specialize h₂ i hi₁ hi₂
+    unfold DArray.get at h₂
+    dsimp at h₂
+    rw [Any.eq_rec_val_iff] at h₂
+    assumption
 
 end DArray
