MemoNat/Attr.lean
@@ -6,31 +6,32 @@ open Lean Meta Elab Tactic Term
 def memoAttrImpl (n : Name) : AttrM Unit := do
   let defn ← getConstInfoDefn n
 
-  let (u, f, drt) <- match defn.value with
+  let (u, f, drt, dmemo, eq_dmemo) <- match defn.value with
     | .app (.app (.app (.app (.app (.const ``WellFounded.fix [_u, u]) dt) drt) _) _) f => do
       match dt with
       | .const `Nat _ => pure ()
-      | _ =>  throwError ("first argument to fix not Nat but" ++ toString dt)
-      pure (u, f, drt)
+      | _ =>  throwError ("first argument to fix not `Nat` but" ++ toString dt)
+
+
+      pure (u, f, drt, ``NatMemo.dmemo, ``NatMemo.fix_eq_dmemo)
     | .lam _ (.const `Nat _) ( .app (.app (.app (.const `Nat.brecOn [u]) drt) _) f) _ => do
-      throwError "definitions using Nat.brecOn are not yet supported"
-      pure (u, f, drt)
+      pure (u, f, drt, ``NatMemo.dmemo_below, ``NatMemo.brecOn_eq_dmemo_below)
     | _ => throwError ("definition right hand side not of expected form: " ++ toString defn.value)
     
   let slow_name := defn.name
   let fast_name := slow_name.append (.mkSimple "fast")
   let eq_name   := slow_name.append (.mkSimple "eq_fast")
-  
+
   addAndCompile (.defnDecl { defn with
     name := fast_name
     -- NB: This declaration has the same type as slow
-    value := mkAppN (mkConst `NatMemo.dmemo [u]) #[drt, f]
+    value := mkAppN (mkConst dmemo [u]) #[drt, f]
   })
 
   addAndCompile (.thmDecl { defn with
     name := eq_name
     type := mkAppN (mkConst `Eq [u]) #[defn.type, mkConst slow_name, mkConst fast_name]
-    value := mkAppN (mkConst `NatMemo.fix_eq_dmemo [u]) #[drt, f]
+    value := mkAppN (mkConst eq_dmemo [u]) #[drt, f]
   })
 
   Lean.Compiler.CSimp.add eq_name AttributeKind.global
